iter

treiber_stack.v
@@ -19,25 +19,35 @@ Definition pop: val :=
   rec: "pop" "s" :=
       let: "hd" := !"s" in
       match: !"hd" with
-        SOME "pair" =>
-        if: CAS "s" "hd" (Snd "pair")
-          then SOME (Fst "pair")
+        SOME "cell" =>
+        if: CAS "s" "hd" (Snd "cell")
+          then SOME (Fst "cell")
           else "pop" "s"
       | NONE => NONE
       end.
 
-Section proof.
-  Context `{!heapG Σ} (N: namespace) (R: val → iProp Σ).
+Definition iter': val :=
+  rec: "iter'" "hd" "f" :=
+      match: !"hd" with
+        NONE => #()
+      | SOME "cell" => "f" (Fst "cell") ;; "iter'" (Snd "cell") "f"
+      end.
 
-  Fixpoint is_stack' (hd: loc) (xs: list val) : iProp Σ :=
+Definition iter: val := λ: "f" "s", iter' (!"s") "f".
+
+Global Opaque new_stack push pop iter' iter.
+
+Section proof.
+  Context `{!heapG Σ} (N: namespace).
+
+  Fixpoint is_stack' (R: val → iProp Σ) (hd: loc) (xs: list val) : iProp Σ :=
     match xs with
     | [] => (∃ q, hd ↦{ q } NONEV)%I
-    | x :: xs => (∃ (hd': loc) q, hd ↦{ q } SOMEV (x, #hd') ★ □ R x ★ is_stack' hd' xs)%I
+    | x :: xs => (∃ (hd': loc) q, hd ↦{ q } SOMEV (x, #hd') ★ R x ★ is_stack' R hd' xs)%I
     end.
 
-  (* how can we prove that it is persistent? *)
-  Lemma dup_is_stack': ∀ xs hd,
-    heap_ctx ★ is_stack' hd xs ⊢ is_stack' hd xs ★ is_stack' hd xs.
+  Lemma dup_is_stack' R `{∀ v, PersistentP (R v)} : ∀ xs hd,
+    heap_ctx ★ is_stack' R hd xs ⊢ is_stack' R hd xs ★ is_stack' R hd xs.
   Proof.
     induction xs as [|y xs' IHxs'].
     - iIntros (hd) "(#? & Hs)".
@@ -48,14 +58,14 @@ Section proof.
       iSplitL "Hhd Hs1"; iExists hd', (q / 2)%Qp; by iFrame.
   Qed.
 
-  Lemma uniq_is_stack':
-    ∀ xs ys hd, heap_ctx ★ is_stack' hd xs ★ is_stack' hd ys ⊢ xs = ys.
+  Lemma uniq_is_stack' R:
+    ∀ xs ys hd, heap_ctx ★ is_stack' R hd xs ★ is_stack' R hd ys ⊢ xs = ys.
   Proof.
     induction xs as [|x xs' IHxs'].
     - induction ys as [|y ys' IHys'].
       + auto.
       + iIntros (hd) "(#? & Hxs & Hys)".
-        simpl. iDestruct "Hys" as (hd' ?) "(Hhd & #Hy & Hys')".
+        simpl. iDestruct "Hys" as (hd' ?) "(Hhd & Hy & Hys')".
         iExFalso. iDestruct "Hxs" as (?) "Hhd'".
         iDestruct (heap_mapsto_op_1 with "[Hhd Hhd']") as "[% _]".
         { iSplitL "Hhd"; done. }
@@ -78,12 +88,12 @@ Section proof.
         by subst.
   Qed.
   
-  Definition is_stack (s: loc) xs: iProp Σ := (∃ hd: loc, s ↦ #hd ★ is_stack' hd xs)%I.
+  Definition is_stack R (s: loc) xs: iProp Σ := (∃ hd: loc, s ↦ #hd ★ is_stack' R hd xs)%I.
 
-  Lemma new_stack_spec:
+  Lemma new_stack_spec R:
     ∀ (Φ: val → iProp Σ),
       heapN ⊥ N →
-      heap_ctx ★ (∀ s, is_stack s [] -★ Φ #s) ⊢ WP new_stack #() {{ Φ }}.
+      heap_ctx ★ (∀ s, is_stack R s [] -★ Φ #s) ⊢ WP new_stack #() {{ Φ }}.
   Proof.
     iIntros (Φ HN) "[#Hh HΦ]". wp_seq.
     wp_bind (ref NONE)%E. wp_alloc l as "Hl".
@@ -92,15 +102,15 @@ Section proof.
     iFrame. by iExists 1%Qp.
   Qed.
 
-  Definition push_triple (s: loc) (x: val) :=
-    atomic_triple (fun xs => □ R x ★ is_stack s xs)%I
-                  (fun xs _ => is_stack s (x :: xs))
+  Definition push_triple R (s: loc) (x: val) :=
+    atomic_triple (fun xs => □ R x ★ is_stack R s xs)%I
+                  (fun xs _ => is_stack R s (x :: xs))
                   (nclose heapN)
                   ⊤
                   (push #s x).
   
-  Lemma push_atomic_spec (s: loc) (x: val) :
-    heapN ⊥ N → heap_ctx ⊢ push_triple s x.
+  Lemma push_atomic_spec R (s: loc) (x: val) :
+    heapN ⊥ N → heap_ctx ⊢ push_triple R s x.
   Proof.
     iIntros (HN) "#?". rewrite /push_triple /atomic_triple.
     iIntros (P Q) "#Hvs".
@@ -126,19 +136,27 @@ Section proof.
       iVsIntro. wp_if. by iApply "IH".
   Qed.
 
-  Definition pop_triple (s: loc) :=
-    atomic_triple (fun xs => is_stack s xs)%I
-                  (fun xs ret => (ret = NONEV ★ xs = [] ★ is_stack s []) ∨
-                                 (∃ x xs', ret = SOMEV x ★ □ R x ★ xs = x :: xs' ★ is_stack s xs'))%I
+  Definition pop_triple_strong R (s: loc) :=
+    atomic_triple (fun xs => is_stack R s xs)%I
+                  (fun xs ret => (ret = NONEV ★ xs = [] ★ is_stack R s []) ∨
+                                 (∃ x xs', ret = SOMEV x ★ □ R x ★ xs = x :: xs' ★ is_stack R s xs'))%I
+                  (nclose heapN)
+                  ⊤
+                  (pop #s).
+
+  Definition pop_triple_weak R (s: loc) :=
+    atomic_triple (fun xs => is_stack R s xs)%I
+                  (fun xs ret => (ret = NONEV ★ xs = [] ★ is_stack R s []) ∨
+                                 (∃ x, ret = SOMEV x ★ R x))%I
                   (nclose heapN)
                   ⊤
                   (pop #s).
   
-  Lemma pop_atomic_spec (s: loc) (x: val) :
-    heapN ⊥ N → heap_ctx ⊢ pop_triple s.
+  Lemma pop_atomic_spec_strong R `{∀ v, PersistentP (R v)} (s: loc) (x: val) :
+    heapN ⊥ N → heap_ctx ⊢ pop_triple_strong R s.
   Proof.
     iIntros (HN) "#?".
-    rewrite /pop_triple /atomic_triple.
+    rewrite /pop_triple_strong /atomic_triple.
     iIntros (P Q) "#Hvs".
     iLöb as "IH". iIntros "!# HP". wp_rec.
     wp_bind (! _)%E.
@@ -172,8 +190,8 @@ Section proof.
             done.
           - simpl. iDestruct "Hhd''" as (hd''' ?) "(Hhd'' & _ & Hxs'')".
             iDestruct (heap_mapsto_op_1 with "[Hhd Hhd'']") as "[% _]".
-            { iSplitL "Hhd"; done. }
-            inversion H0. (* FIXME: bad naming *) subst.
+            { iSplitL "Hhd"; done. } 
+            inversion H1. (* FIXME: bad naming *) subst.
             iDestruct (uniq_is_stack' with "[Hxs1 Hxs'']") as "%"; first by iFrame. subst.
             repeat (iSplitR "Hxs1 Hs"; first done).
             iExists hd'''. by iFrame.
@@ -184,5 +202,88 @@ Section proof.
         { iExists hd''. by iFrame. }
         iVsIntro. wp_if. by iApply "IH".
   Qed.
-      
+
+  (* FIXME: Code dup with pop_atomic_spec_strong *)
+  Lemma pop_atomic_spec_weak R (s: loc) (x: val) :
+    heapN ⊥ N → heap_ctx ⊢ pop_triple_weak R s.
+  Proof.
+    iIntros (HN) "#?".
+    rewrite /pop_triple_strong /atomic_triple.
+    iIntros (P Q) "#Hvs".
+    iLöb as "IH". iIntros "!# HP". wp_rec.
+    wp_bind (! _)%E.
+    iVs ("Hvs" with "HP") as (xs) "[Hxs Hvs']".
+    destruct xs as [|y' xs'].
+    - simpl. iDestruct "Hxs" as (hd) "[Hs Hhd]".
+      wp_load. iDestruct "Hvs'" as "[_ Hvs']".
+      iDestruct "Hhd" as (q) "[Hhd Hhd']".
+      iVs ("Hvs'" $! NONEV with "[-Hhd]") as "HQ".
+      { iLeft. iSplit=>//. iSplit=>//.
+        iExists hd. iFrame. rewrite /is_stack'. eauto. }
+      iVsIntro. wp_let. wp_load. wp_match.
+      iVsIntro. by iExists [].
+    - simpl. iDestruct "Hxs" as (hd) "[Hs Hhd]".
+      simpl. iDestruct "Hhd" as (hd' q) "([Hhd Hhd'] & Hy' & Hxs')".
+      wp_load. iDestruct "Hvs'" as "[Hvs' _]".
+      iVs ("Hvs'" with "[-Hhd]") as "HP".
+      { iExists hd. iFrame. iExists hd', (q / 2)%Qp. by iFrame. }
+      iVsIntro. wp_let. wp_load. wp_match. wp_proj.
+      wp_bind (CAS _ _ _). iVs ("Hvs" with "HP") as (xs) "[Hxs Hvs']".
+      iDestruct "Hxs" as (hd'') "[Hs Hhd'']".
+      destruct (decide (hd = hd'')) as [->|Hneq].
+      + wp_cas_suc. iDestruct "Hvs'" as "[_ Hvs']".
+        iVs ("Hvs'" $! (SOMEV y') with "[-]") as "HQ".
+        { iRight. rewrite /is_stack. iExists y'.
+          destruct xs as [|x' xs''].
+          - simpl. iDestruct "Hhd''" as (?) "H".
+            iExFalso. iDestruct (heap_mapsto_op_1 with "[Hhd H]") as "[% _]".
+            { iSplitL "Hhd"; done. }
+            done.
+          - simpl. iDestruct "Hhd''" as (hd''' ?) "(Hhd'' & Hx' & Hxs'')".
+            iDestruct (heap_mapsto_op_1 with "[Hhd Hhd'']") as "[% _]".
+            { iSplitL "Hhd"; done. } 
+            inversion H0. (* FIXME: bad naming *) subst.
+            eauto.
+        }
+        iVsIntro. wp_if. wp_proj. eauto.
+      + wp_cas_fail. iDestruct "Hvs'" as "[Hvs' _]".
+        iVs ("Hvs'" with "[-]") as "HP".
+        { iExists hd''. by iFrame. }
+        iVsIntro. wp_if. by iApply "IH".
+  Qed.
+
+  Lemma iter_spec' R R' (f: val) :
+    ∀ xs (hd: loc),
+      heapN ⊥ N → (∀ x: val, {{ R x }} f x {{ _, R' x }} ) →
+      heap_ctx ★ is_stack' R hd xs ⊢ WP iter' #hd f {{ _,  is_stack' R' hd xs }}.
+  Proof.
+    induction xs as [|x xs' IHxs'].
+    - iIntros (hd HN Hf) "[#? Hs]".
+      simpl. iDestruct "Hs" as (?) "Hhd".
+      wp_rec. wp_let. wp_load. wp_match. eauto.
+    - iIntros (hd HN Hf) "[#? Hs]".
+      simpl. iDestruct "Hs" as (hd' q) "(Hhd & Hx & Hxs')".
+      wp_rec. wp_let. wp_load. wp_match. wp_proj.
+      wp_bind (f _). iApply wp_wand_r.
+      iSplitL "Hx"; first by iApply Hf.
+      iIntros (?) "Hx". wp_seq.
+      iApply wp_wand_r.
+      iSplitL "Hxs'". wp_proj.
+      { iApply (IHxs' with "[Hxs']")=>//. by iFrame. }
+      iIntros (?) "Hs".
+      iExists hd', q. by iFrame.
+  Qed.
+
+  Lemma iter_spec R R' (s: loc) xs (f: val) :
+    heapN ⊥ N → (∀ x: val, {{ R x }} f x {{ _, R' x }} ) →
+    heap_ctx ★ is_stack R s xs ⊢ WP iter f #s {{ _,  is_stack R' s xs }}.
+  Proof.
+    iIntros (HN Hf) "[#? Hs]".
+    wp_seq. wp_let. iDestruct "Hs" as (hd) "[Hs Hhd]".
+    wp_load. iApply wp_wand_r. iSplitL "Hhd".
+    { iApply (iter_spec' with "[Hhd]")=>//. by iFrame. }
+    iIntros (?) "Hhd'".
+    iExists hd. by iFrame.
+  Qed.
+  
 End proof.
